rename stpd2 to stpd

dev2016/dot.v
@@ -393,7 +393,7 @@ Inductive vtp(*possible types*) : nat(*pack count*) -> venv -> id -> ty -> nat(*
 
 Definition has_typed GH G1 x T1 := exists n, has_type GH G1 x T1 n.
 
-Definition stpd2 GH G1 T1 T2 := exists n, stp GH G1 T1 T2 n.
+Definition stpd GH G1 T1 T2 := exists n, stp GH G1 T1 T2 n.
 
 Definition htpd GH G1 x T1 := exists n, htp GH G1 x T1 n.
 
@@ -410,41 +410,41 @@ Ltac ep := match goal with
 
 Ltac eu := match goal with
              | H: has_typed _ _ _ _ |- _ => destruct H as [? H]
-             | H: stpd2 _ _ _ _ |- _ => destruct H as [? H]
+             | H: stpd _ _ _ _ |- _ => destruct H as [? H]
              | H: htpd _ _ _ _ |- _ => destruct H as [? H]
              | H: vtpd _ _ _ _ |- _ => destruct H as [? H]
              | H: vtpdd _ _ _ _ |- _ => destruct H as [? [? [H ?]]]
            end.
 
-Lemma stpd2_bot: forall GH G1 T,
+Lemma stpd_bot: forall GH G1 T,
     closed (length GH) (length G1) 0 T ->
-    stpd2 GH G1 TBot T.
+    stpd GH G1 TBot T.
 Proof. intros. exists 1. eauto. Qed.
-Lemma stpd2_top: forall GH G1 T,
+Lemma stpd_top: forall GH G1 T,
     closed (length GH) (length G1) 0 T ->
-    stpd2 GH G1 T TTop.
+    stpd GH G1 T TTop.
 Proof. intros. exists 1. eauto. Qed.
-Lemma stpd2_fun: forall GH G1 l T1 T2 T3 T4 T2' T4',
+Lemma stpd_fun: forall GH G1 l T1 T2 T3 T4 T2' T4',
     T2' = (open 0 (TVar false (length GH)) T2) ->
     T4' = (open 0 (TVar false (length GH)) T4) ->
     closed (length GH) (length G1) 1 T2 ->
     closed (length GH) (length G1) 1 T4 ->
-    stpd2 GH G1 T3 T1 ->
-    stpd2 (T3::GH) G1 T2' T4' ->
-    stpd2 GH G1 (TFun l T1 T2) (TFun l T3 T4).
+    stpd GH G1 T3 T1 ->
+    stpd (T3::GH) G1 T2' T4' ->
+    stpd GH G1 (TFun l T1 T2) (TFun l T3 T4).
 Proof. intros. repeat eu. eexists. eauto. Qed.
-Lemma stpd2_mem: forall GH G1 l T1 T2 T3 T4,
-    stpd2 GH G1 T3 T1 ->
-    stpd2 GH G1 T2 T4 ->
-    stpd2 GH G1 (TMem l T1 T2) (TMem l T3 T4).
+Lemma stpd_mem: forall GH G1 l T1 T2 T3 T4,
+    stpd GH G1 T3 T1 ->
+    stpd GH G1 T2 T4 ->
+    stpd GH G1 (TMem l T1 T2) (TMem l T3 T4).
 Proof. intros. repeat eu. eexists. eauto. Qed.
 
 
 
-Lemma stpd2_trans: forall GH G1 T1 T2 T3,
-    stpd2 GH G1 T1 T2 ->
-    stpd2 GH G1 T2 T3 ->
-    stpd2 GH G1 T1 T3.
+Lemma stpd_trans: forall GH G1 T1 T2 T3,
+    stpd GH G1 T1 T2 ->
+    stpd GH G1 T2 T3 ->
+    stpd GH G1 T1 T3.
 Proof. intros. repeat eu. eexists. eauto. Qed.
 
 
@@ -460,7 +460,7 @@ Hint Constructors htp.
 Hint Constructors has_type.
 
 Hint Unfold has_typed.
-Hint Unfold stpd2.
+Hint Unfold stpd.
 Hint Unfold vtpd.
 Hint Unfold vtpdd.
 
@@ -875,14 +875,14 @@ Lemma stp_closed2 : forall GH G1 T1 T2 n1,
                       closed (length GH) (length G1) 0 T2.
 Proof. intros. edestruct all_closed. destruct H1. eapply H1. eauto. eauto. Qed.
 
-Lemma stpd2_closed1 : forall GH G1 T1 T2,
-                      stpd2 GH G1 T1 T2 ->
+Lemma stpd_closed1 : forall GH G1 T1 T2,
+                      stpd GH G1 T1 T2 ->
                       closed (length GH) (length G1) 0 T1.
 Proof. intros. eu. eapply stp_closed1. eauto. Qed.
 
 
-Lemma stpd2_closed2 : forall GH G1 T1 T2,
-                      stpd2 GH G1 T1 T2 ->
+Lemma stpd_closed2 : forall GH G1 T1 T2,
+                      stpd GH G1 T1 T2 ->
                       closed (length GH) (length G1) 0 T2.
 Proof. intros. eu. eapply stp_closed2. eauto. Qed.
 
@@ -912,22 +912,22 @@ Proof.
   - destruct (beq_nat j i); eauto.
 Qed.
 
-Lemma stpd2_refl_aux: forall n GH G1 T1,
+Lemma stpd_refl_aux: forall n GH G1 T1,
   closed (length GH) (length G1) 0 T1 ->
   tsize T1 < n ->
-  stpd2 GH G1 T1 T1.
+  stpd GH G1 T1 T1.
 Proof.
   intros n. induction n; intros; try omega.
   inversion H; subst; simpl in H0.
   - Case "bot". exists 1. eauto.
   - Case "top". exists 1. eauto.
-  - Case "fun". eapply stpd2_fun; eauto.
+  - Case "fun". eapply stpd_fun; eauto.
     eapply IHn; eauto; omega.
     eapply IHn; eauto.
     simpl. apply closed_open. simpl. eapply closed_upgrade_gh. eauto. omega.
     econstructor. omega.
     rewrite <- open_preserves_size. omega.
-  - Case "mem". eapply stpd2_mem; try eapply IHn; eauto; try omega.
+  - Case "mem". eapply stpd_mem; try eapply IHn; eauto; try omega.
   - Case "var0". exists 1. eauto.
   - Case "var1". exists 1. eauto.
   - Case "varb". omega.
@@ -949,22 +949,22 @@ Grab Existential Variables.
 apply 0.
 Qed.
 
-Lemma stpd2_refl: forall GH G1 T1,
+Lemma stpd_refl: forall GH G1 T1,
   closed (length GH) (length G1) 0 T1 ->
-  stpd2 GH G1 T1 T1.
+  stpd GH G1 T1 T1.
 Proof.
-  intros. apply stpd2_refl_aux with (n:=S (tsize T1)); eauto.
+  intros. apply stpd_refl_aux with (n:=S (tsize T1)); eauto.
 Qed.
 
-Lemma stpd2_reg1 : forall GH G1 T1 T2,
-                      stpd2 GH G1 T1 T2 ->
-                      stpd2 GH G1 T1 T1.
-Proof. intros. eapply stpd2_refl. eapply stpd2_closed1. eauto. Qed.
+Lemma stpd_reg1 : forall GH G1 T1 T2,
+                      stpd GH G1 T1 T2 ->
+                      stpd GH G1 T1 T1.
+Proof. intros. eapply stpd_refl. eapply stpd_closed1. eauto. Qed.
 
-Lemma stpd2_reg2 : forall GH G1 T1 T2,
-                      stpd2 GH G1 T1 T2 ->
-                      stpd2 GH G1 T2 T2.
-Proof. intros. eapply stpd2_refl. eapply stpd2_closed2. eauto. Qed.
+Lemma stpd_reg2 : forall GH G1 T1 T2,
+                      stpd GH G1 T1 T2 ->
+                      stpd GH G1 T2 T2.
+Proof. intros. eapply stpd_refl. eapply stpd_closed2. eauto. Qed.
 
 
 
@@ -1279,7 +1279,7 @@ Lemma stp_subst_narrow0: forall n, forall GH G1 T1 T2 TX x n2,
    (forall GH (T3 : ty) (n1 : nat),
       htp (GH++[TX]) G1 0 T3 n1 -> n1 < n ->
       exists m2, vtpd m2 G1 x (substt x T3)) ->
-   stpd2 (map (substt x) GH) G1 (substt x T1) (substt x T2).
+   stpd (map (substt x) GH) G1 (substt x T1) (substt x T2).
 Proof.
   intros n. induction n. intros. omega.
   intros ? ? ? ? ? ? ? ? ? ? narrowX.
@@ -1303,7 +1303,7 @@ Proof.
         destruct A as [GL0 [? ?]]. subst GL.
         assert (htpd (map (substt x) GH0) G1 (xi-1) (substt x T3)) as AA.
         eapply IHni. eauto. eauto. omega. omega.
-        assert (stpd2 (map (substt x) GL0) G1 (substt x T3) (substt x T0)) as BB.
+        assert (stpd (map (substt x) GL0) G1 (substt x T3) (substt x T0)) as BB.
         eapply IHn. eauto. eauto. omega. { intros. eapply narrowX. eauto. eauto. }
         eu. eu. repeat eexists. eapply htp_sub. eauto. eauto.
         (* - *)
@@ -1326,11 +1326,11 @@ Proof.
   (* main logic *)
   inversion H.
   - Case "bot". subst.
-    eapply stpd2_bot; eauto. rewrite map_length. simpl. eapply closed_subst0. rewrite app_length in H2. simpl in H2. eapply H2. eauto.
+    eapply stpd_bot; eauto. rewrite map_length. simpl. eapply closed_subst0. rewrite app_length in H2. simpl in H2. eapply H2. eauto.
   - Case "top". subst.
-    eapply stpd2_top; eauto. rewrite map_length. simpl. eapply closed_subst0. rewrite app_length in H2. simpl in H2. eapply H2. eauto.
+    eapply stpd_top; eauto. rewrite map_length. simpl. eapply closed_subst0. rewrite app_length in H2. simpl in H2. eapply H2. eauto.
   - Case "fun". subst.
-    eapply stpd2_fun. eauto. eauto.
+    eapply stpd_fun. eauto. eauto.
     rewrite map_length. eapply closed_subst0. rewrite app_length in *. simpl in *. eauto. omega.
     rewrite map_length. eapply closed_subst0. rewrite app_length in *. simpl in *. eauto. omega.
     eapply IHn; eauto. omega.
@@ -1341,7 +1341,7 @@ Proof.
     rewrite map_length. rewrite app_length in *. eassumption.
     omega. omega. eauto.
   - Case "mem". subst.
-    eapply stpd2_mem. eapply IHn; eauto. omega. eapply IHn; eauto. omega.
+    eapply stpd_mem. eapply IHn; eauto. omega. eapply IHn; eauto. omega.
 
 
   - Case "varx". subst.
@@ -1355,11 +1355,11 @@ Proof.
       assert (x0 <> 0). eapply beq_nat_false_iff. eauto.
       repeat eexists. unfold substt. simpl. rewrite E. eapply stp_varax. rewrite map_length. rewrite app_length in H2. simpl in H2. omega.
   - Case "ssel1". subst.
-    assert (substt x T2 = T2) as R. eapply subst_closed_id. eapply stpd2_closed2 with (GH:=[]). eauto.
+    assert (substt x T2 = T2) as R. eapply subst_closed_id. eapply stpd_closed2 with (GH:=[]). eauto.
     eexists. eapply stp_strong_sel1. eauto. eauto. rewrite R. eauto.
 
   - Case "ssel2". subst.
-    assert (substt x T1 = T1) as R. eapply subst_closed_id. eapply stpd2_closed1 with (GH:=[]). eauto.
+    assert (substt x T1 = T1) as R. eapply subst_closed_id. eapply stpd_closed1 with (GH:=[]). eauto.
     eexists. eapply stp_strong_sel2. eauto. eauto. rewrite R. eauto.
 
   - Case "sel1". subst. (* invert htp to vtp and create strong_sel node *)
@@ -1404,31 +1404,31 @@ Proof.
     rewrite app_length in H6. simpl in H6. eauto. eapply closed_subst0. rewrite map_length. eauto. eauto.
 
   - Case "and11".
-    assert (stpd2 (map (substt x) GH) G1 (substt x T0) (substt x T2)). eapply IHn. eauto. eauto. omega. eauto.
+    assert (stpd (map (substt x) GH) G1 (substt x T0) (substt x T2)). eapply IHn. eauto. eauto. omega. eauto.
     eu. eexists. eapply stp_and11. eauto. eapply closed_subst0. rewrite app_length in H3. rewrite map_length. eauto. eauto.
   - Case "and12".
-    assert (stpd2 (map (substt x) GH) G1 (substt x T3) (substt x T2)). eapply IHn. eauto. eauto. omega. eauto.
+    assert (stpd (map (substt x) GH) G1 (substt x T3) (substt x T2)). eapply IHn. eauto. eauto. omega. eauto.
     eu. eexists. eapply stp_and12. eauto. eapply closed_subst0. rewrite app_length in H3. rewrite map_length. eauto. eauto.
   - Case "and2".
-    assert (stpd2 (map (substt x) GH) G1 (substt x T1) (substt x T0)). eapply IHn. eauto. eauto. omega. eauto.
-    assert (stpd2 (map (substt x) GH) G1 (substt x T1) (substt x T3)). eapply IHn. eauto. eauto. omega. eauto.
+    assert (stpd (map (substt x) GH) G1 (substt x T1) (substt x T0)). eapply IHn. eauto. eauto. omega. eauto.
+    assert (stpd (map (substt x) GH) G1 (substt x T1) (substt x T3)). eapply IHn. eauto. eauto. omega. eauto.
     eu. eu. eexists. eapply stp_and2. eauto. eauto.
 
   - Case "or21".
-    assert (stpd2 (map (substt x) GH) G1 (substt x T1) (substt x T0)). eapply IHn. eauto. eauto. omega. eauto.
+    assert (stpd (map (substt x) GH) G1 (substt x T1) (substt x T0)). eapply IHn. eauto. eauto. omega. eauto.
     eu. eexists. eapply stp_or21. eauto. eapply closed_subst0. rewrite app_length in H3. rewrite map_length. eauto. eauto.
   - Case "or22".
-    assert (stpd2 (map (substt x) GH) G1 (substt x T1) (substt x T3)). eapply IHn. eauto. eauto. omega. eauto.
+    assert (stpd (map (substt x) GH) G1 (substt x T1) (substt x T3)). eapply IHn. eauto. eauto. omega. eauto.
     eu. eexists. eapply stp_or22. eauto. eapply closed_subst0. rewrite app_length in H3. rewrite map_length. eauto. eauto.
   - Case "or1".
-    assert (stpd2 (map (substt x) GH) G1 (substt x T0) (substt x T2)). eapply IHn. eauto. eauto. omega. eauto.
-    assert (stpd2 (map (substt x) GH) G1 (substt x T3) (substt x T2)). eapply IHn. eauto. eauto. omega. eauto.
+    assert (stpd (map (substt x) GH) G1 (substt x T0) (substt x T2)). eapply IHn. eauto. eauto. omega. eauto.
+    assert (stpd (map (substt x) GH) G1 (substt x T3) (substt x T2)). eapply IHn. eauto. eauto. omega. eauto.
     eu. eu. eexists. eapply stp_or1. eauto. eauto.
 
   - Case "trans".
-    assert (stpd2 (map (substt x) GH) G1 (substt x T1) (substt x T3)).
+    assert (stpd (map (substt x) GH) G1 (substt x T1) (substt x T3)).
     eapply IHn; eauto. omega.
-    assert (stpd2 (map (substt x) GH) G1 (substt x T3) (substt x T2)).
+    assert (stpd (map (substt x) GH) G1 (substt x T3) (substt x T2)).
     eapply IHn; eauto. omega.
     eu. eu. repeat eexists. eapply stp_trans. eauto. eauto.
 
@@ -1468,7 +1468,7 @@ Proof.
     assert (vtpdd m G1 x (substt x T1)) as A.
     eapply IHnl. eauto. eauto. eauto. eauto. omega. eauto.
     eu.
-    assert (stpd2 [] G1 (substt x T1) (substt x T2)) as B.
+    assert (stpd [] G1 (substt x T1) (substt x T2)) as B.
     erewrite subst_closed_id. erewrite subst_closed_id. eexists. eassumption.
     eapply stp_closed2 in H6. simpl in H6. eapply H6.
     eapply stp_closed1 in H6. simpl in H6. eapply H6.
@@ -1485,7 +1485,7 @@ Proof.
     assert (vtpdd m G1 x (substt x T1)) as A.
     eapply IHnl. eauto. eauto. eauto. eauto. omega. eauto.
     eu.
-    assert (stpd2 (map (substt x) []) G1 (substt x T1) (substt x T2)) as B.
+    assert (stpd (map (substt x) []) G1 (substt x T1) (substt x T2)) as B.
     eapply stp_subst_narrow0. eauto. eauto. eauto. {
       intros. eapply IHnl in H. eu. repeat eexists. eauto. eauto. eauto. eauto. omega. eauto.
     }
@@ -2135,15 +2135,15 @@ Lemma stp_narrow_aux: forall n,
   forall GH1 GH0 GH' TX1 TX2,
     GH=GH1++[TX2]++GH0 ->
     GH'=GH1++[TX1]++GH0 ->
-    stpd2 GH0 G TX1 TX2 ->
+    stpd GH0 G TX1 TX2 ->
     htpd GH' G x T) /\
   (forall GH G T1 T2 n0,
   stp GH G T1 T2 n0 -> n0 <= n ->
   forall GH1 GH0 GH' TX1 TX2,
     GH=GH1++[TX2]++GH0 ->
     GH'=GH1++[TX1]++GH0 ->
-    stpd2 GH0 G TX1 TX2 ->
-    stpd2 GH' G T1 T2).
+    stpd GH0 G TX1 TX2 ->
+    stpd GH' G T1 T2).
 Proof.
   intros n.
   induction n.
@@ -2214,16 +2214,16 @@ Proof.
     assert (length GH' = length GH) as EGHLEN by solve [
       subst; repeat rewrite app_length; simpl; reflexivity
     ].
-    + SCase "bot". eapply stpd2_bot. rewrite EGHLEN; assumption.
-    + SCase "top". eapply stpd2_top. rewrite EGHLEN; assumption.
-    + SCase "fun". eapply stpd2_fun.
+    + SCase "bot". eapply stpd_bot. rewrite EGHLEN; assumption.
+    + SCase "top". eapply stpd_top. rewrite EGHLEN; assumption.
+    + SCase "fun". eapply stpd_fun.
       reflexivity. reflexivity.
       rewrite EGHLEN; assumption. rewrite EGHLEN; assumption.
       eapply IHn_stp; try eassumption. omega.
       eapply IHn_stp with (GH1:=(T4::GH1)); try eassumption.
       rewrite EGHLEN. eauto. omega.
       subst. simpl. reflexivity. subst. simpl. reflexivity.
-    + SCase "mem". eapply stpd2_mem.
+    + SCase "mem". eapply stpd_mem.
       eapply IHn_stp; try eassumption. omega.
       eapply IHn_stp; try eassumption. omega.
     + SCase "varx". eexists. eapply stp_varx. omega.
@@ -2294,7 +2294,7 @@ Qed.
 Lemma stp_narrow: forall TX1 TX2 GH0 G T1 T2 n nx,
   stp ([TX2]++GH0) G T1 T2 n ->
   stp GH0 G TX1 TX2 nx ->
-  stpd2 ([TX1]++GH0) G T1 T2.
+  stpd ([TX1]++GH0) G T1 T2.
 Proof.
   intros. eapply stp_narrow_aux. eapply H. reflexivity.
   instantiate(3:=nil). simpl. reflexivity. simpl. reflexivity.
@@ -2362,7 +2362,7 @@ Proof.
   - Case "fun". inversion H0; subst; invty.
     + SCase "top". repeat eexists. eapply vtp_top. eapply index_max. eauto. eauto.
     + SCase "fun". invty. subst.
-      assert (stpd2 [T8] G1 (open 0 (TVar false 0) T0) (open 0 (TVar false 0) T5)) as A. {
+      assert (stpd [T8] G1 (open 0 (TVar false 0) T0) (open 0 (TVar false 0) T5)) as A. {
         eapply stp_narrow. simpl. eassumption. simpl. eassumption.
       }
       destruct A as [na A].
@@ -2455,7 +2455,7 @@ Proof.
       eu. repeat eexists. eapply vtp_sel. eauto. eauto. eauto. eauto.
     + SCase "sel1".
       assert (closed (length ([]:tenv)) (length G1) 0 (TSel (TVar false x0) l1)) as A.
-      eapply stpd2_closed2. eauto.
+      eapply stpd_closed2. eauto.
       simpl in A. inversion A. inversion H12. omega.
     + SCase "selx".
       eauto.
@@ -2572,7 +2572,7 @@ Inductive step : venv -> tm -> venv -> tm -> Prop :=
 Lemma stp_subst_narrow_z: forall GH0 TX G1 T1 T2 x m n1 n2,
   stp (GH0 ++ [TX]) G1 T1 T2 n2 ->
   vtp m G1 x (substt x TX) n1 ->
-  stpd2 (map (substt x) GH0) G1 (substt x T1) (substt x T2).
+  stpd (map (substt x) GH0) G1 (substt x T1) (substt x T2).
 Proof.
   intros.
   edestruct stp_subst_narrow0. eauto. eapply vtp_closed1. eauto. eauto.
@@ -2631,8 +2631,8 @@ Proof.
       unfold substt in *. simpl in HC. inversion HC; subst.
       inversion H6; subst. eauto.
     }
-    assert (stpd2 [] G1 (substt x T11) (substt x T11)) as A. {
-      eapply stpd2_refl. eauto.
+    assert (stpd [] G1 (substt x T11) (substt x T11)) as A. {
+      eapply stpd_refl. eauto.
     }
     eu.
     destruct Hds as [dsa Hdsa]. simpl in Hdsa.
@@ -2655,12 +2655,12 @@ Proof.
       eapply closed_open. eapply closed_upgrade_gh. eauto. omega.
       econstructor. omega.
     }
-    assert (stpd2 [] G1 (substt x T11) (substt x T11)) as A. {
-      eapply stpd2_refl. eauto.
+    assert (stpd [] G1 (substt x T11) (substt x T11)) as A. {
+      eapply stpd_refl. eauto.
     }
     eu.
-    assert (stpd2 [(substt x T11)] G1 (open 0 (TVar false 0) (substt x T12)) (open 0 (TVar false 0) (substt x T12))) as B. {
-      eapply stpd2_refl. eauto.
+    assert (stpd [(substt x T11)] G1 (open 0 (TVar false 0) (substt x T12)) (open 0 (TVar false 0) (substt x T12))) as B. {
+      eapply stpd_refl. eauto.
     }
     eu.
     destruct Hds as [dsa Hdsa]. simpl in Hdsa.
@@ -2869,7 +2869,7 @@ Qed.
 Lemma stp_subst_narrow: forall GH0 TX G1 T1 T2 x m n1 n2,
   stp (GH0 ++ [TX]) G1 T1 T2 n2 ->
   vtp m G1 x TX n1 ->
-  stpd2 (map (substt x) GH0) G1 (substt x T1) (substt x T2).
+  stpd (map (substt x) GH0) G1 (substt x T1) (substt x T2).
 Proof.
   intros. eapply stp_subst_narrow_z. eauto.
   erewrite subst_closed_id. eauto. eapply vtp_closed in H0. eauto.
@@ -3012,7 +3012,7 @@ Proof.
     assert ((exists x : id, t0 = tvar true x) \/
                (exists (G' : venv) (t' : tm) n2,
                   step G1 t0 (G'++G1) t' /\ has_type [] (G'++G1) t' T1 n2)) as HH.
-    eapply IHhas_type; eauto. change 0 with (length ([]:tenv)) at 1. eapply stpd2_closed1; eauto.
+    eapply IHhas_type; eauto. change 0 with (length ([]:tenv)) at 1. eapply stpd_closed1; eauto.
     destruct HH.
     + SCase "val".
       ev. subst. left. eexists. eauto.
